start solving constraint systems

src/Syntax/ImportResolver.thy
@@ -9,6 +9,10 @@ theory ImportResolver
     Syntax.Digraph
     Syntax.Constraints
     Syntax.Errors
+    Syntax.FileIO
+    Syntax.Lexer
+    Syntax.Parser
+    Syntax.Desugarer
 begin
 
 fun bind_sum :: \<open>'a + 'b \<Rightarrow> ('b \<Rightarrow> 'a + 'c) \<Rightarrow> 'a + 'c\<close>
@@ -33,11 +37,69 @@ datatype module_origin =
   CommandLine
 | InSource position
 
-type_synonym mod_list = \<open>(module_origin \<times> String.literal) list\<close>
+type_synonym mod_list = \<open>(module_origin \<times> String.literal list) list\<close>
 
 fun origin_to_position :: \<open>module_origin \<Rightarrow> position option\<close>
 where \<open>origin_to_position CommandLine = None\<close>
     | \<open>origin_to_position (InSource pos) = Some pos\<close>
+
+fun pos_or :: \<open>module_origin \<Rightarrow> 'a \<Rightarrow> position + 'a\<close>
+where \<open>pos_or CommandLine x = Inr x\<close>
+    | \<open>pos_or (InSource p) _ = Inl p\<close>
+
+datatype interface =
+  Iface \<open>String.literal \<rightharpoonup> interface\<close>
+
+type_synonym namespaces = \<open>String.literal \<rightharpoonup> interface option\<close>
+
+type_synonym global_state = \<open>system list \<times> mod_list \<times> namespaces \<times> modules \<times> import_graph\<close>
+
+type_synonym 'a resolver = \<open>[global_state, registered_files] \<Rightarrow> ((String.literal diagnostic + global_state \<times> 'a) \<times> registered_files) io\<close>
+
+fun bind_resolver :: \<open>'a resolver \<Rightarrow> ('a \<Rightarrow> 'b resolver) \<Rightarrow> 'b resolver\<close>
+where \<open>bind_resolver r f st fs = do {
+         (res, fs) \<leftarrow> r st fs;
+         case res of
+           Inl diag \<Rightarrow> IO.return (Inl diag, fs)
+         | Inr (st, x) \<Rightarrow> f x st fs
+       }\<close>
+adhoc_overloading bind bind_resolver
+
+definition return :: \<open>'a \<Rightarrow> 'a resolver\<close>
+where \<open>return x st fs = IO.return (Inr (st, x), fs)\<close>
+
+definition throw :: \<open>String.literal diagnostic \<Rightarrow> 'a resolver\<close>
+where \<open>throw diag _ fs = IO.return (Inl diag, fs)\<close>
+
+definition append_system :: \<open>system \<Rightarrow> unit resolver\<close>
+where \<open>append_system s \<equiv> (\<lambda>(ss, ml, ns, ms, g) fs. IO.return (Inr ((s # ss, ml, ns, ms, g), ()), fs))\<close>
+
+definition set_system :: \<open>[nat, system] \<Rightarrow> unit resolver\<close>
+where \<open>set_system n s = (\<lambda>(ss, ml, ns, ms, g) fs. IO.return (Inr ((ss[n := s], ml, ns, ms, g), ()), fs))\<close>
+
+definition insert_interface :: \<open>[String.literal, interface option] \<Rightarrow> unit resolver\<close>
+where \<open>insert_interface name iface \<equiv> (\<lambda>(ss, ml, ns, ms, g) fs. IO.return (Inr ((ss, ml, ns(name \<mapsto> iface), ms, g), ()), fs))\<close>
+
+definition insert_module :: \<open>[String.literal, AST.module located] \<Rightarrow> unit resolver\<close>
+where \<open>insert_module name m \<equiv> (\<lambda>(ss, ml, ns, ms, g) fs. IO.return (Inr ((ss, ml, ns, ms(name \<mapsto> m), g), ()), fs))\<close>
+
+definition register_module :: \<open>[String.literal list, module_origin] \<Rightarrow> unit resolver\<close>
+where \<open>register_module m orig \<equiv> (\<lambda>(ss, ml, ns, ms, g) fs. IO.return (Inr ((ss, (orig, m) # ml, ns, ms, g), ()), fs))\<close>
+
+definition insert_dependency :: \<open>[String.literal, String.literal] \<Rightarrow> unit resolver\<close>
+where \<open>insert_dependency a b \<equiv> (\<lambda>(ss, ml, ns, ms, g) fs. IO.return (Inr ((ss, ml, ns, ms, add_edge (a, b) g), ()), fs))\<close>
+
+definition get :: \<open>global_state resolver\<close>
+where \<open>get \<equiv> (\<lambda>st fs. IO.return (Inr (st, st), fs))\<close>
+
+definition lift_io :: \<open>'a io \<Rightarrow> 'a resolver\<close>
+where \<open>lift_io act \<equiv> (\<lambda>st fs. do { x \<leftarrow> act; IO.return (Inr (st, x), fs) })\<close>
+
+definition lift_sum :: \<open>String.literal diagnostic + 'a \<Rightarrow> 'a resolver\<close>
+where \<open>lift_sum res \<equiv> (\<lambda>st fs. IO.return (map_sum id (Pair st) res, fs))\<close>
+
+fun contains :: \<open>String.literal \<Rightarrow> interface \<Rightarrow> bool\<close>
+where \<open>contains x (Iface binds) = (binds x \<noteq> None)\<close>
 
 (************************************************)
 
@@ -45,10 +107,10 @@ axiomatization
     parse_module_name :: \<open>position option \<Rightarrow> String.literal \<Rightarrow> String.literal diagnostic + String.literal list\<close>
 and mk_constraint_system :: \<open>String.literal list \<Rightarrow> String.literal list \<Rightarrow> system\<close>
 
-fun try_mk_constraints_for_module :: \<open>String.literal list \<Rightarrow> module_origin \<Rightarrow> String.literal \<Rightarrow> (String.literal diagnostic + system)\<close>
+fun try_mk_constraints_for_module :: \<open>String.literal list \<Rightarrow> module_origin \<Rightarrow> String.literal \<Rightarrow> (String.literal diagnostic + system \<times> String.literal list)\<close>
 where \<open>try_mk_constraints_for_module idirs orig m = do {
          parts \<leftarrow> parse_module_name (origin_to_position orig) m;
-         Inr (mk_constraint_system idirs parts)
+         Inr (mk_constraint_system idirs parts, parts)
        }\<close>
 
 code_printing
@@ -62,7 +124,7 @@ code_printing
 {-# LANGUAGE MultiParamTypeClasses #-}
 {-# OPTIONS_GHC -Wno-orphans #-}
 
-module ImportResolver (Formula (..), Constraint, System, parseModuleName, mkConstraintSystem) where
+module ImportResolver (Formula (..), Namespace (..), Constraint, System, parseModuleName, mkConstraintSystem) where
 
 import Data.Bifunctor (first)
 import Data.Functor ((<&>))
@@ -79,8 +141,8 @@ data Namespace
   deriving (Show)
 
 data Formula
-  = Top
-  | Bottom
+  = Top Formula
+  | Bottom Formula
   | Exists FilePath
   | In String Namespace
   deriving (Show)
@@ -161,38 +223,136 @@ code_reserved Haskell ImportResolver parseModuleName mkConstraintSystem
  * *)
 (* TODO: add the imports of the new module to be processed (if not already processed) *)
 
-fun make_initial_constraint_system :: \<open>String.literal list \<Rightarrow> mod_list \<Rightarrow> (String.literal diagnostic + global_system)\<close>
-where \<open>make_initial_constraint_system _ [] = Inr []\<close>
+fun make_initial_constraint_system :: \<open>[String.literal list, (module_origin \<times> String.literal) list] \<Rightarrow> (String.literal diagnostic + system list \<times> mod_list)\<close>
+where \<open>make_initial_constraint_system _ [] = Inr ([], [])\<close>
     | \<open>make_initial_constraint_system idirs ((orig, m) # ms) = do {
-         csts \<leftarrow> try_mk_constraints_for_module idirs orig m;
-         sys \<leftarrow> make_initial_constraint_system idirs ms;
-         Inr (csts # sys)
+         (csts, m) \<leftarrow> try_mk_constraints_for_module idirs orig m;
+         (sys, ms) \<leftarrow> make_initial_constraint_system idirs ms;
+         Inr (csts # sys, (orig, m) # ms)
        }\<close>
 
-fun try_solve_system_incrementally :: \<open>import_graph \<Rightarrow> global_system \<Rightarrow> mod_list \<Rightarrow> ((String.literal diagnostic + modules) \<times> import_graph \<times> registered_files \<times> mod_list) io\<close>
-where \<open>try_solve_system_incrementally g [] [] = IO.return (Inr Map.empty, g, Map.empty, [])\<close>
-      (* Erroneous cases: module import has no associated constraint *)
-    | \<open>try_solve_system_incrementally g ([] # _) ((CommandLine, m) # ms) =
-         IO.return (Inl (mk_cannot_import_cli_module_error m), g, Map.empty, (CommandLine, m) # ms)\<close>
-    | \<open>try_solve_system_incrementally g ([] # _) ((InSource p, m) # ms) =
-         IO.return undefined\<close>
-      (* Still at least one constraint to solve *)
-    | \<open>try_solve_system_incrementally g (c # cs) ((orig, m) # ms) = do {
-         IO.return undefined
+fun find_unsolved_system :: \<open>unit \<Rightarrow> ((nat \<times> system) option) resolver\<close>
+where \<open>find_unsolved_system () = do {
+         (ss, _, _, _, _) \<leftarrow> get;
+         case [(i, s) \<leftarrow> enumerate 0 ss. \<not> is_fully_solved s] of
+           [] \<Rightarrow> return None
+         | c # _ \<Rightarrow> return (Some c)
        }\<close>
-      (* Inconsistent state: more constraints than modules, or more modules than constraints *)
-    | \<open>try_solve_system_incrementally _ _ _ = undefined\<close>
 
-fun parse_and_resolve_modules :: \<open>String.literal list \<Rightarrow> String.literal list \<Rightarrow> ((String.literal diagnostic + modules \<times> module_order) \<times> registered_files) io\<close>
+text \<open>
+  Returns a two-level \<open>option\<close> :
+  \<^item> The first \<open>option\<close> level tells whether the interface has been generated, or if it is
+    held back by additional constraints;
+  \<^item> The second \<open>option\<close> level tells whether an access could be performed within the generated interface.
+    For example, imagine that you need to check that \<open>x \<in> (MOD f)∷y\<close>, but \<open>MOD f\<close> does not contain \<open>y\<close>.
+    Then \<open>Some None\<close> will be returned.
+\<close>
+fun try_generate_interface :: \<open>namespace \<Rightarrow> (interface option option \<times> nat) resolver\<close>
+where \<open>try_generate_interface _ = undefined\<close>
+
+fun try_solve_constraint :: \<open>constraint \<Rightarrow> (constraint \<times> nat) resolver\<close>
+where \<open>try_solve_constraint [] = return ([], 0)\<close>
+    | \<open>try_solve_constraint (Top f # fs) = do {
+         (fs, n) \<leftarrow> try_solve_constraint fs;
+         return (Top f # fs, n)
+       }\<close>
+    | \<open>try_solve_constraint (Bottom f # fs) = do {
+         (fs, n) \<leftarrow> try_solve_constraint fs;
+         return (Bottom f # fs, n)
+       }\<close>
+    | \<open>try_solve_constraint (Exists path # fs) = do {
+         file_exists \<leftarrow> lift_io (does_file_exist path);
+         if file_exists
+           then do {
+             (_, _, ms, _) \<leftarrow> get;
+             (case ms path of
+               None \<Rightarrow> do {
+                 content \<leftarrow> lift_io (read_file path);
+                 (tokens, _) \<leftarrow> lift_sum (run_lexer path content);
+                 (cst, _) \<leftarrow> lift_sum (run_parser path tokens);
+                 (ast, _) \<leftarrow> lift_sum (run_desugarer cst);
+                 insert_module path ast
+               }
+             | Some _ \<Rightarrow> return ());
+             (fs, n) \<leftarrow> try_solve_constraint fs;
+             return (Top (Exists path) # fs, n)
+           }
+           else return (Bottom (Exists path) # fs, 0)
+        }\<close>
+     | \<open>try_solve_constraint (In x n # fs) = do {
+          (iface, i) \<leftarrow> try_generate_interface n;
+          case iface of
+            None \<Rightarrow> return (In x n # fs, i)
+          | Some None \<Rightarrow> return (Bottom (In x n) # fs, i)
+          | Some (Some iface) \<Rightarrow>
+              if contains x iface
+                then do {
+                  (fs, k) \<leftarrow> try_solve_constraint fs;
+                  return (Top (In x n) # fs, i + k)
+                }
+                else return (Bottom (In x n) # fs, i)
+        }\<close>
+
+fun try_solve_each_constraint :: \<open>system \<Rightarrow> (system \<times> nat) resolver\<close>
+where \<open>try_solve_each_constraint [] = return ([], 0)\<close>
+    | \<open>try_solve_each_constraint (c # cs) = do {
+         (c, i) \<leftarrow> if is_solved c then return (c, 0) else try_solve_constraint c;
+         (cs, n) \<leftarrow> try_solve_each_constraint cs;
+         return (c # cs, i + n)
+       }\<close>
+
+fun try_solve_system :: \<open>[nat, system] \<Rightarrow> unit resolver\<close>
+where \<open>try_solve_system i s = do {
+         (cs, n) \<leftarrow> try_solve_each_constraint s;
+         set_system (i + n) cs
+       }\<close>
+
+function try_solve_systems_incrementally :: \<open>unit \<Rightarrow> unit resolver\<close>
+where \<open>try_solve_systems_incrementally _ = do {
+         sys \<leftarrow> find_unsolved_system ();
+         case sys of
+           None \<Rightarrow> return ()
+         | Some (i, s) \<Rightarrow> try_solve_system i s \<bind> try_solve_systems_incrementally
+       }\<close>
+by pat_completeness auto
+
+termination try_solve_systems_incrementally
+  sorry
+(* NOTE: need to prove termination for \<open>try_solve_systems_incrementally\<close> to get code equations *)
+
+fun check_all_systems :: \<open>system list \<Rightarrow> mod_list \<Rightarrow> unit resolver\<close>
+where \<open>check_all_systems [] _ = return ()\<close>
+    | \<open>check_all_systems (s # ss) ((orig, m) # ms) =
+         (case [c \<leftarrow> s. is_true c] of
+           [] \<Rightarrow> throw (mk_cannot_resolve_import_error (pos_or orig m) (map (the \<circ> only_false_constraint) s))
+         | (a # b # cs) \<Rightarrow> throw undefined
+         | [_] \<Rightarrow> check_all_systems ss ms)\<close>
+    (* Inconsistent state: all systems must have an associated module *)
+    | \<open>check_all_systems _ _ = undefined\<close>
+(* TODO: fetch the position of the import associated to this system.
+         also fetch the name of the import if it is a CLI import (i.e. no position).
+
+         \<open>mk_cannot_resolve_import_error\<close> must take a \<open>String.literal + position\<close> as argument. *)
+
+fun check_final_systems :: \<open>unit \<Rightarrow> unit resolver\<close>
+where \<open>check_final_systems () = do {
+         (ss, ml, _, _, _) \<leftarrow> get;
+         check_all_systems ss ml
+       }\<close>
+
+fun parse_and_resolve_modules :: \<open>[String.literal list, String.literal list] \<Rightarrow> ((String.literal diagnostic + modules \<times> module_order) \<times> registered_files) io\<close>
 where \<open>parse_and_resolve_modules idirs mods = do {
-         let mods' = map (Pair CommandLine) mods;
-         let sys = make_initial_constraint_system idirs mods';
+         let mods = map (Pair CommandLine) mods;
+         let sys = make_initial_constraint_system idirs mods;
          case sys of
            Inl diag \<Rightarrow> IO.return (Inl diag, Map.empty)
-         | Inr sys \<Rightarrow> do {
-             (res, g, files, _) \<leftarrow> try_solve_system_incrementally Digraph.empty sys mods';
+         | Inr (sys, mods) \<Rightarrow> do {
+             (res, files) \<leftarrow> (do {
+               try_solve_systems_incrementally ();
+               check_final_systems ()
+             }) (sys, mods, Map.empty, Map.empty, Digraph.empty) Map.empty;
              let res = do {
-                   mods \<leftarrow> res;
+                   ((_, _, _, mods, g), ()) \<leftarrow> res;
                    map_sum undefined (Pair mods) (topsort g)
                  };
              IO.return (res, files)
@@ -203,6 +363,6 @@ hide_type module_origin
 hide_const CommandLine InSource
 
 (* Prevent using \<open>bind_sum\<close> outside this theory. *)
-hide_const bind_sum
+hide_const bind_sum bind_resolver return
 
 end
