src/Syntax/Constraints.thy
@@ -8,8 +8,8 @@ datatype namespace =
 | Access namespace String.literal
 
 datatype formula =
-  Top
-| Bottom
+  Top formula
+| Bottom formula
 | Exists String.literal
 | In String.literal namespace
 
@@ -19,11 +19,38 @@ text \<open>
 type_synonym constraint = \<open>formula list\<close>
 
 text \<open>
-  An OR-separated list of constraints.
+  A XOR-separated list of constraints.
 \<close>
 type_synonym system = \<open>constraint list\<close>
 
 type_synonym global_system = \<open>system list\<close>
+
+(****************************************************)
+
+fun is_bottom :: \<open>formula \<Rightarrow> bool\<close>
+where \<open>is_bottom (Bottom _) = True\<close>
+    | \<open>is_bottom _ = False\<close>
+
+fun is_top :: \<open>formula \<Rightarrow> bool\<close>
+where \<open>is_top (Top _) = True\<close>
+    | \<open>is_top _ = False\<close>
+
+definition is_false :: \<open>constraint \<Rightarrow> bool\<close>
+where \<open>is_false c \<equiv> list_ex is_bottom c\<close>
+
+definition is_true :: \<open>constraint \<Rightarrow> bool\<close>
+where \<open>is_true c \<equiv> list_all is_top c\<close>
+
+definition is_solved :: \<open>constraint \<Rightarrow> bool\<close>
+where \<open>is_solved c \<equiv> (is_false c \<or> is_true c)\<close>
+
+definition is_fully_solved :: \<open>system \<Rightarrow> bool\<close>
+where \<open>is_fully_solved s \<equiv> list_all is_solved s\<close>
+
+fun only_false_constraint :: \<open>constraint \<Rightarrow> formula option\<close>
+where \<open>only_false_constraint [] = None\<close>
+    | \<open>only_false_constraint (Bottom f # _) = Some f\<close>
+    | \<open>only_false_constraint (_ # fs) = only_false_constraint fs\<close>
 
 (****************************************************)
 
