src/Syntax/Desugarer.thy
@@ -1,0 +1,16 @@
+theory Desugarer
+  imports
+    Main
+
+    Located.At
+
+    Diagnose.Diagnostic
+
+    Syntax.CST
+    Syntax.AST
+begin
+
+fun run_desugarer :: \<open>CST.module located \<Rightarrow> String.literal diagnostic + AST.module located \<times> String.literal diagnostic\<close>
+where \<open>run_desugarer _ = undefined\<close>
+
+end
