src/Syntax/FileIO.thy
@@ -1,0 +1,22 @@
+theory FileIO
+  imports
+    Main
+    Hello_World.IO
+begin
+
+axiomatization
+    does_file_exist :: \<open>String.literal \<Rightarrow> bool io\<close>
+and read_file :: \<open>String.literal \<Rightarrow> String.literal io\<close>
+
+code_printing
+  constant does_file_exist \<rightharpoonup> (Haskell) "FileIO.doesFileExist"
+| constant read_file \<rightharpoonup> (Haskell) "FileIO.readFile"
+
+| code_module FileIO \<rightharpoonup> (Haskell) \<open>
+module FileIO (module Export) where
+
+import System.Directory as Export (doesFileExist)
+import Prelude as Export (readFile)
+\<close>
+
+end
